pcuic/theories/PCUICPredExtra.v
@@ -1,0 +1,536 @@
+(* Distributed under the terms of the MIT license.   *)
+Set Warnings "-notation-overridden".
+Require Import ssreflect ssrbool.
+From Coq Require Import Bool List Utf8 ZArith Lia Morphisms String.
+From MetaCoq.Template Require Import config utils.
+From MetaCoq.PCUIC Require Import PCUICAst PCUICAstUtils PCUICSize
+  PCUICLiftSubst PCUICSigmaCalculus PCUICUnivSubst PCUICTyping PCUICReduction
+  PCUICSubstitution PCUICReflect PCUICClosed PCUICParallelReduction
+  PCUICPattern PCUICInduction PCUICRW.
+
+Require Import monad_utils.
+Import MonadNotation.
+
+(* Type-valued relations. *)
+Require Import CRelationClasses.
+Require Import Equations.Prop.DepElim.
+From Equations Require Import Equations.
+
+Set Default Goal Selector "!".
+
+Local Set Keyed Unification.
+Set Asymmetric Patterns.
+
+(* All the rewrite rules of a rewrite_decl *)
+Definition all_rewrite_rules (rd : rewrite_decl) :=
+  rd.(prules) ++ rd.(rules).
+
+Section ParallelReductionExtra.
+
+  Context (Σ : global_env).
+
+  (* Potential extra rules, might be redundant *)
+  Context (extra : option (kername × rewrite_decl)).
+
+  Inductive pred1_extra (Γ Γ' : context) : term -> term -> Type :=
+  (** Reductions *)
+  (** Beta *)
+  | predx_beta na t0 t1 b0 b1 a0 a1 :
+      pred1_extra Γ Γ' t0 t1 ->
+      pred1_extra (Γ ,, vass na t0) (Γ' ,, vass na t1) b0 b1 -> pred1_extra Γ Γ' a0 a1 ->
+      pred1_extra Γ Γ' (tApp (tLambda na t0 b0) a0) (subst10 a1 b1)
+
+  (** Let *)
+  | predx_zeta na d0 d1 t0 t1 b0 b1 :
+      pred1_extra Γ Γ' t0 t1 ->
+      pred1_extra Γ Γ' d0 d1 -> pred1_extra (Γ ,, vdef na d0 t0) (Γ' ,, vdef na d1 t1) b0 b1 ->
+      pred1_extra Γ Γ' (tLetIn na d0 t0 b0) (subst10 d1 b1)
+
+  (** Local variables *)
+  | predx_rel_def_unfold i body :
+      All2_local_env (on_decl pred1_extra) Γ Γ' ->
+      option_map decl_body (nth_error Γ' i) = Some (Some body) ->
+      pred1_extra Γ Γ' (tRel i) (lift0 (S i) body)
+
+  | predx_rel_refl i :
+      All2_local_env (on_decl pred1_extra) Γ Γ' ->
+      pred1_extra Γ Γ' (tRel i)  (tRel i)
+
+  (** Case *)
+  | predx_iota ind pars c u args0 args1 p brs0 brs1 :
+      All2_local_env (on_decl pred1_extra) Γ Γ' ->
+      All2 (pred1_extra Γ Γ') args0 args1 ->
+      All2 (on_Trel_eq (pred1_extra Γ Γ') snd fst) brs0 brs1 ->
+      pred1_extra Γ Γ' (tCase (ind, pars) p (mkApps (tConstruct ind c u) args0) brs0)
+            (iota_red pars c args1 brs1)
+
+  (** Fix unfolding, with guard *)
+  | predx_fix mfix0 mfix1 idx args0 args1 narg fn :
+      All2_local_env (on_decl pred1_extra) Γ Γ' ->
+      All2_local_env (on_decl (on_decl_over pred1_extra Γ Γ')) (fix_context mfix0) (fix_context mfix1) ->
+      All2_prop2_eq Γ Γ' (Γ ,,, fix_context mfix0) (Γ' ,,, fix_context mfix1)
+                    dtype dbody (fun x => (dname x, rarg x)) pred1_extra mfix0 mfix1 ->
+      unfold_fix mfix1 idx = Some (narg, fn) ->
+      is_constructor narg args0 = true ->
+      All2 (pred1_extra Γ Γ') args0 args1 ->
+      pred1_extra Γ Γ' (mkApps (tFix mfix0 idx) args0) (mkApps fn args1)
+
+  (** CoFix-case unfolding *)
+  | predx_cofix_case ip p0 p1 mfix0 mfix1 idx args0 args1 narg fn brs0 brs1 :
+      All2_local_env (on_decl pred1_extra) Γ Γ' ->
+      All2_local_env (on_decl (on_decl_over pred1_extra Γ Γ')) (fix_context mfix0) (fix_context mfix1) ->
+      All2_prop2_eq Γ Γ' (Γ ,,, fix_context mfix0) (Γ' ,,, fix_context mfix1)
+                    dtype dbody (fun x => (dname x, rarg x)) pred1_extra mfix0 mfix1 ->
+      unfold_cofix mfix1 idx = Some (narg, fn) ->
+      All2 (pred1_extra Γ Γ') args0 args1 ->
+      pred1_extra Γ Γ' p0 p1 ->
+      All2 (on_Trel_eq (pred1_extra Γ Γ') snd fst) brs0 brs1 ->
+      pred1_extra Γ Γ' (tCase ip p0 (mkApps (tCoFix mfix0 idx) args0) brs0)
+            (tCase ip p1 (mkApps fn args1) brs1)
+
+  (** CoFix-proj unfolding *)
+  | predx_cofix_proj p mfix0 mfix1 idx args0 args1 narg fn :
+      All2_local_env (on_decl pred1_extra) Γ Γ' ->
+      All2_local_env (on_decl (on_decl_over pred1_extra Γ Γ')) (fix_context mfix0) (fix_context mfix1) ->
+      All2_prop2_eq Γ Γ' (Γ ,,, fix_context mfix0) (Γ' ,,, fix_context mfix1)
+                    dtype dbody (fun x => (dname x, rarg x)) pred1_extra mfix0 mfix1 ->
+      unfold_cofix mfix1 idx = Some (narg, fn) ->
+      All2 (pred1_extra Γ Γ') args0 args1 ->
+      pred1_extra Γ Γ' (tProj p (mkApps (tCoFix mfix0 idx) args0))
+            (tProj p (mkApps fn args1))
+
+  (** Symbols and rewrite rules  *)
+
+  | predx_symb k n u :
+      All2_local_env (on_decl pred1_extra) Γ Γ' ->
+      pred1_extra Γ Γ' (tSymb k n u) (tSymb k n u)
+
+  | predx_rewrite_rule k ui decl n r s s' :
+      All2_local_env (on_decl pred1_extra) Γ Γ' ->
+      declared_symbol Σ k decl ->
+      nth_error decl.(rules) n = Some r ->
+      All2 (pred1_extra Γ Γ') s s' ->
+      let ss := symbols_subst k 0 ui #|decl.(symbols)| in
+      untyped_subslet Γ s (subst_context ss 0 r.(pat_context)) ->
+      let lhs := subst0 s (subst ss #|s| (lhs r)) in
+      let rhs := subst0 s' (subst ss #|s| (rhs r)) in
+      pred1_extra Γ Γ' lhs rhs
+
+  | predx_par_rewrite_rule k ui decl n r s s' :
+      All2_local_env (on_decl pred1_extra) Γ Γ' ->
+      declared_symbol Σ k decl ->
+      nth_error decl.(prules) n = Some r ->
+      All2 (pred1_extra Γ Γ') s s' ->
+      let ss := symbols_subst k 0 ui #|decl.(symbols)| in
+      untyped_subslet Γ s (subst_context ss 0 r.(pat_context)) ->
+      let lhs := subst0 s (subst ss #|s| (lhs r)) in
+      let rhs := subst0 s' (subst ss #|s| (rhs r)) in
+      pred1_extra Γ Γ' lhs rhs
+
+  | predx_extra_rewrite_rule k ui decl n r s s' :
+      All2_local_env (on_decl pred1_extra) Γ Γ' ->
+      extra = Some (k, decl) →
+      nth_error (all_rewrite_rules decl) n = Some r ->
+      All2 (pred1_extra Γ Γ') s s' ->
+      let ss := symbols_subst k 0 ui #|decl.(symbols)| in
+      untyped_subslet Γ s (subst_context ss 0 r.(pat_context)) ->
+      let lhs := subst0 s (subst ss #|s| (lhs r)) in
+      let rhs := subst0 s' (subst ss #|s| (rhs r)) in
+      pred1_extra Γ Γ' lhs rhs
+
+  (** Constant unfolding *)
+
+  | predx_delta c decl body (isdecl : declared_constant Σ c decl) u :
+      All2_local_env (on_decl pred1_extra) Γ Γ' ->
+      decl.(cst_body) = Some body ->
+      pred1_extra Γ Γ' (tConst c u) (subst_instance_constr u body)
+
+  | predx_const c u :
+      All2_local_env (on_decl pred1_extra) Γ Γ' ->
+      pred1_extra Γ Γ' (tConst c u) (tConst c u)
+
+  (** Proj *)
+  | predx_proj i pars narg k u args0 args1 arg1 :
+      All2_local_env (on_decl pred1_extra) Γ Γ' ->
+      All2 (pred1_extra Γ Γ') args0 args1 ->
+      nth_error args1 (pars + narg) = Some arg1 ->
+      pred1_extra Γ Γ' (tProj (i, pars, narg) (mkApps (tConstruct i k u) args0)) arg1
+
+  (** Congruences *)
+  | predx_abs na M M' N N' : pred1_extra Γ Γ' M M' -> pred1_extra (Γ ,, vass na M) (Γ' ,, vass na M') N N' ->
+                            pred1_extra Γ Γ' (tLambda na M N) (tLambda na M' N')
+  | predx_app M0 M1 N0 N1 :
+      pred1_extra Γ Γ' M0 M1 ->
+      pred1_extra Γ Γ' N0 N1 ->
+      pred1_extra Γ Γ' (tApp M0 N0) (tApp M1 N1)
+            (* do not handle mkApps yet *)
+
+  | predx_letin na d0 d1 t0 t1 b0 b1 :
+      pred1_extra Γ Γ' d0 d1 -> pred1_extra Γ Γ' t0 t1 -> pred1_extra (Γ ,, vdef na d0 t0) (Γ' ,, vdef na d1 t1) b0 b1 ->
+      pred1_extra Γ Γ' (tLetIn na d0 t0 b0) (tLetIn na d1 t1 b1)
+
+  | predx_case ind p0 p1 c0 c1 brs0 brs1 :
+      pred1_extra Γ Γ' p0 p1 ->
+      pred1_extra Γ Γ' c0 c1 ->
+      All2 (on_Trel_eq (pred1_extra Γ Γ') snd fst) brs0 brs1 ->
+      pred1_extra Γ Γ' (tCase ind p0 c0 brs0) (tCase ind p1 c1 brs1)
+
+  | predx_proj_congr p c c' :
+      pred1_extra Γ Γ' c c' -> pred1_extra Γ Γ' (tProj p c) (tProj p c')
+
+  | predx_fix_congr mfix0 mfix1 idx :
+      All2_local_env (on_decl pred1_extra) Γ Γ' ->
+      All2_local_env (on_decl (on_decl_over pred1_extra Γ Γ')) (fix_context mfix0) (fix_context mfix1) ->
+      All2_prop2_eq Γ Γ' (Γ ,,, fix_context mfix0) (Γ' ,,, fix_context mfix1)
+                    dtype dbody (fun x => (dname x, rarg x)) pred1_extra mfix0 mfix1 ->
+      pred1_extra Γ Γ' (tFix mfix0 idx) (tFix mfix1 idx)
+
+  | predx_cofix_congr mfix0 mfix1 idx :
+      All2_local_env (on_decl pred1_extra) Γ Γ' ->
+      All2_local_env (on_decl (on_decl_over pred1_extra Γ Γ')) (fix_context mfix0) (fix_context mfix1) ->
+      All2_prop2_eq Γ Γ' (Γ ,,, fix_context mfix0) (Γ' ,,, fix_context mfix1)
+                    dtype dbody (fun x => (dname x, rarg x)) pred1_extra mfix0 mfix1 ->
+      pred1_extra Γ Γ' (tCoFix mfix0 idx) (tCoFix mfix1 idx)
+
+  | predx_prod na M0 M1 N0 N1 : pred1_extra Γ Γ' M0 M1 -> pred1_extra (Γ ,, vass na M0) (Γ' ,, vass na M1) N0 N1 ->
+                               pred1_extra Γ Γ' (tProd na M0 N0) (tProd na M1 N1)
+
+  | evar_pred ev l l' :
+      All2_local_env (on_decl pred1_extra) Γ Γ' ->
+      All2 (pred1_extra Γ Γ') l l' -> pred1_extra Γ Γ' (tEvar ev l) (tEvar ev l')
+
+  | predx_atom_refl t :
+      All2_local_env (on_decl pred1_extra) Γ Γ' ->
+      pred_atom t -> pred1_extra Γ Γ' t t.
+
+  Lemma pred1_extra_ind_all_ctx :
+    forall (P : forall (Γ Γ' : context) (t t0 : term), Type)
+           (Pctx : forall (Γ Γ' : context), Type),
+      let P' Γ Γ' x y := ((pred1_extra Γ Γ' x y) * P Γ Γ' x y)%type in
+      (forall Γ Γ', All2_local_env (on_decl pred1_extra) Γ Γ' -> All2_local_env (on_decl P) Γ Γ' -> Pctx Γ Γ') ->
+      (forall (Γ Γ' : context) (na : name) (t0 t1 b0 b1 a0 a1 : term),
+          pred1_extra (Γ ,, vass na t0) (Γ' ,, vass na t1) b0 b1 -> P (Γ ,, vass na t0) (Γ' ,, vass na t1) b0 b1 ->
+          pred1_extra Γ Γ' t0 t1 -> P Γ Γ' t0 t1 ->
+          pred1_extra Γ Γ' a0 a1 -> P Γ Γ' a0 a1 -> P Γ Γ' (tApp (tLambda na t0 b0) a0) (b1 {0 := a1})) ->
+      (forall (Γ Γ' : context) (na : name) (d0 d1 t0 t1 b0 b1 : term),
+          pred1_extra Γ Γ' t0 t1 -> P Γ Γ' t0 t1 ->
+          pred1_extra Γ Γ' d0 d1 -> P Γ Γ' d0 d1 ->
+          pred1_extra (Γ ,, vdef na d0 t0) (Γ' ,, vdef na d1 t1) b0 b1 ->
+          P (Γ ,, vdef na d0 t0) (Γ' ,, vdef na d1 t1) b0 b1 -> P Γ Γ' (tLetIn na d0 t0 b0) (b1 {0 := d1})) ->
+      (forall (Γ Γ' : context) (i : nat) (body : term),
+          All2_local_env (on_decl pred1_extra) Γ Γ' ->
+          Pctx Γ Γ' ->
+          option_map decl_body (nth_error Γ' i) = Some (Some body) ->
+          P Γ Γ' (tRel i) (lift0 (S i) body)) ->
+      (forall (Γ Γ' : context) (i : nat),
+          All2_local_env (on_decl pred1_extra) Γ Γ' ->
+          Pctx Γ Γ' ->
+          P Γ Γ' (tRel i) (tRel i)) ->
+      (forall (Γ Γ' : context) (ind : inductive) (pars c : nat) (u : Instance.t) (args0 args1 : list term)
+              (p : term) (brs0 brs1 : list (nat * term)),
+          All2_local_env (on_decl pred1_extra) Γ Γ' ->
+          Pctx Γ Γ' ->
+          All2 (P' Γ Γ') args0 args1 ->
+          All2_prop_eq Γ Γ' snd fst P' brs0 brs1 ->
+          P Γ Γ' (tCase (ind, pars) p (mkApps (tConstruct ind c u) args0) brs0) (iota_red pars c args1 brs1)) ->
+      (forall (Γ Γ' : context) (mfix0 mfix1 : mfixpoint term) (idx : nat) (args0 args1 : list term) (narg : nat) (fn : term),
+          All2_local_env (on_decl pred1_extra) Γ Γ' ->
+          Pctx Γ Γ' ->
+          All2_local_env (on_decl (on_decl_over pred1_extra Γ Γ')) (fix_context mfix0) (fix_context mfix1) ->
+          All2_local_env (on_decl (on_decl_over P Γ Γ')) (fix_context mfix0) (fix_context mfix1) ->
+          All2_prop2_eq Γ Γ' (Γ ,,, fix_context mfix0) (Γ' ,,, fix_context mfix1) dtype dbody
+                        (fun x => (dname x, rarg x)) P' mfix0 mfix1 ->
+          unfold_fix mfix1 idx = Some (narg, fn) ->
+          is_constructor narg args0 = true ->
+          All2 (P' Γ Γ') args0 args1 ->
+          P Γ Γ' (mkApps (tFix mfix0 idx) args0) (mkApps fn args1)) ->
+      (forall (Γ Γ' : context) (ip : inductive * nat) (p0 p1 : term) (mfix0 mfix1 : mfixpoint term) (idx : nat)
+              (args0 args1 : list term) (narg : nat) (fn : term) (brs0 brs1 : list (nat * term)),
+          All2_local_env (on_decl pred1_extra) Γ Γ' ->
+          Pctx Γ Γ' ->
+          All2_local_env (on_decl (on_decl_over pred1_extra Γ Γ')) (fix_context mfix0) (fix_context mfix1) ->
+          All2_local_env (on_decl (on_decl_over P Γ Γ')) (fix_context mfix0) (fix_context mfix1) ->
+          All2_prop2_eq Γ Γ' (Γ ,,, fix_context mfix0) (Γ' ,,, fix_context mfix1) dtype dbody
+                        (fun x => (dname x, rarg x)) P' mfix0 mfix1 ->
+          unfold_cofix mfix1 idx = Some (narg, fn) ->
+          All2 (P' Γ Γ') args0 args1 ->
+          pred1_extra Γ Γ' p0 p1 ->
+          P Γ Γ' p0 p1 ->
+          All2_prop_eq Γ Γ' snd fst P' brs0 brs1 ->
+          P Γ Γ' (tCase ip p0 (mkApps (tCoFix mfix0 idx) args0) brs0) (tCase ip p1 (mkApps fn args1) brs1)) ->
+      (forall (Γ Γ' : context) (p : projection) (mfix0 mfix1 : mfixpoint term)
+         (idx : nat) (args0 args1 : list term)
+         (narg : nat) (fn : term),
+          All2_local_env (on_decl pred1_extra) Γ Γ' ->
+          Pctx Γ Γ' ->
+          All2_local_env (on_decl (on_decl_over pred1_extra Γ Γ')) (fix_context mfix0) (fix_context mfix1) ->
+          All2_local_env (on_decl (on_decl_over P Γ Γ')) (fix_context mfix0) (fix_context mfix1) ->
+          All2_prop2_eq Γ Γ' (Γ ,,, fix_context mfix0) (Γ' ,,, fix_context mfix1) dtype dbody
+                        (fun x => (dname x, rarg x)) P' mfix0 mfix1 ->
+          unfold_cofix mfix1 idx = Some (narg, fn) ->
+          All2 (P' Γ Γ') args0 args1 ->
+          P Γ Γ' (tProj p (mkApps (tCoFix mfix0 idx) args0)) (tProj p (mkApps fn args1))) ->
+      (forall (Γ Γ' : context) (c : kername) (n : nat) (u : Instance.t),
+          All2_local_env (on_decl pred1_extra) Γ Γ' ->
+          Pctx Γ Γ' ->
+          P Γ Γ' (tSymb c n u) (tSymb c n u)) ->
+      (forall (Γ Γ' : context) k ui decl n r s s',
+          All2_local_env (on_decl pred1_extra) Γ Γ' ->
+          Pctx Γ Γ' ->
+          declared_symbol Σ k decl ->
+          nth_error decl.(rules) n = Some r ->
+          All2 (P' Γ Γ') s s' ->
+          let ss := symbols_subst k 0 ui #|decl.(symbols)| in
+          untyped_subslet Γ s (subst_context ss 0 r.(pat_context)) ->
+          let lhs := subst0 s (subst ss #|s| (lhs r)) in
+          let rhs := subst0 s' (subst ss #|s| (rhs r)) in
+          P Γ Γ' lhs rhs
+      ) ->
+      (forall (Γ Γ' : context) k ui decl n r s s',
+          All2_local_env (on_decl pred1_extra) Γ Γ' ->
+          Pctx Γ Γ' ->
+          declared_symbol Σ k decl ->
+          nth_error decl.(prules) n = Some r ->
+          All2 (P' Γ Γ') s s' ->
+          let ss := symbols_subst k 0 ui #|decl.(symbols)| in
+          untyped_subslet Γ s (subst_context ss 0 r.(pat_context)) ->
+          let lhs := subst0 s (subst ss #|s| (lhs r)) in
+          let rhs := subst0 s' (subst ss #|s| (rhs r)) in
+          P Γ Γ' lhs rhs
+      ) ->
+      (forall (Γ Γ' : context) k ui decl n r s s',
+          All2_local_env (on_decl pred1_extra) Γ Γ' ->
+          Pctx Γ Γ' ->
+          extra = Some (k, decl) →
+          nth_error (all_rewrite_rules decl) n = Some r ->
+          All2 (P' Γ Γ') s s' ->
+          let ss := symbols_subst k 0 ui #|decl.(symbols)| in
+          untyped_subslet Γ s (subst_context ss 0 r.(pat_context)) ->
+          let lhs := subst0 s (subst ss #|s| (lhs r)) in
+          let rhs := subst0 s' (subst ss #|s| (rhs r)) in
+          P Γ Γ' lhs rhs
+      ) ->
+      (forall (Γ Γ' : context) (c : kername) (decl : constant_body) (body : term),
+          All2_local_env (on_decl pred1_extra) Γ Γ' ->
+          Pctx Γ Γ' ->
+          declared_constant Σ c decl ->
+          forall u : Instance.t, cst_body decl = Some body ->
+                                        P Γ Γ' (tConst c u) (subst_instance_constr u body)) ->
+      (forall (Γ Γ' : context) c (u : Instance.t),
+          All2_local_env (on_decl pred1_extra) Γ Γ' ->
+          Pctx Γ Γ' ->
+          P Γ Γ' (tConst c u) (tConst c u)) ->
+      (forall (Γ Γ' : context) (i : inductive) (pars narg : nat) (k : nat) (u : Instance.t)
+              (args0 args1 : list term) (arg1 : term),
+          All2_local_env (on_decl pred1_extra) Γ Γ' ->
+          Pctx Γ Γ' ->
+          All2 (pred1_extra Γ Γ') args0 args1 ->
+          All2 (P Γ Γ') args0 args1 ->
+          nth_error args1 (pars + narg) = Some arg1 ->
+          P Γ Γ' (tProj (i, pars, narg) (mkApps (tConstruct i k u) args0)) arg1) ->
+      (forall (Γ Γ' : context) (na : name) (M M' N N' : term),
+          pred1_extra Γ Γ' M M' ->
+          P Γ Γ' M M' -> pred1_extra (Γ,, vass na M) (Γ' ,, vass na M') N N' ->
+          P (Γ,, vass na M) (Γ' ,, vass na M') N N' -> P Γ Γ' (tLambda na M N) (tLambda na M' N')) ->
+      (forall (Γ Γ' : context) (M0 M1 N0 N1 : term),
+          pred1_extra Γ Γ' M0 M1 -> P Γ Γ' M0 M1 -> pred1_extra Γ Γ' N0 N1 ->
+          P Γ Γ' N0 N1 -> P Γ Γ' (tApp M0 N0) (tApp M1 N1)) ->
+      (forall (Γ Γ' : context) (na : name) (d0 d1 t0 t1 b0 b1 : term),
+          pred1_extra Γ Γ' d0 d1 ->
+          P Γ Γ' d0 d1 ->
+          pred1_extra Γ Γ' t0 t1 ->
+          P Γ Γ' t0 t1 ->
+          pred1_extra (Γ,, vdef na d0 t0) (Γ',,vdef na d1 t1) b0 b1 ->
+          P (Γ,, vdef na d0 t0) (Γ',,vdef na d1 t1) b0 b1 -> P Γ Γ' (tLetIn na d0 t0 b0) (tLetIn na d1 t1 b1)) ->
+      (forall (Γ Γ' : context) (ind : inductive * nat) (p0 p1 c0 c1 : term) (brs0 brs1 : list (nat * term)),
+          pred1_extra Γ Γ' p0 p1 ->
+          P Γ Γ' p0 p1 ->
+          pred1_extra Γ Γ' c0 c1 ->
+          P Γ Γ' c0 c1 -> All2_prop_eq Γ Γ' snd fst P' brs0 brs1 ->
+          P Γ Γ' (tCase ind p0 c0 brs0) (tCase ind p1 c1 brs1)) ->
+      (forall (Γ Γ' : context) (p : projection) (c c' : term), pred1_extra Γ Γ' c c' -> P Γ Γ' c c' -> P Γ Γ' (tProj p c) (tProj p c')) ->
+
+      (forall (Γ Γ' : context) (mfix0 : mfixpoint term) (mfix1 : list (def term)) (idx : nat),
+          All2_local_env (on_decl pred1_extra) Γ Γ' ->
+          Pctx Γ Γ' ->
+          All2_local_env (on_decl (on_decl_over pred1_extra Γ Γ')) (fix_context mfix0) (fix_context mfix1) ->
+          All2_local_env (on_decl (on_decl_over P Γ Γ')) (fix_context mfix0) (fix_context mfix1) ->
+          All2_prop2_eq Γ Γ' (Γ ,,, fix_context mfix0) (Γ' ,,, fix_context mfix1)
+                        dtype dbody (fun x => (dname x, rarg x)) P' mfix0 mfix1 ->
+          P Γ Γ' (tFix mfix0 idx) (tFix mfix1 idx)) ->
+
+      (forall (Γ Γ' : context) (mfix0 : mfixpoint term) (mfix1 : list (def term)) (idx : nat),
+          All2_local_env (on_decl pred1_extra) Γ Γ' ->
+          Pctx Γ Γ' ->
+          All2_local_env (on_decl (on_decl_over pred1_extra Γ Γ')) (fix_context mfix0) (fix_context mfix1) ->
+          All2_local_env (on_decl (on_decl_over P Γ Γ')) (fix_context mfix0) (fix_context mfix1) ->
+          All2_prop2_eq Γ Γ' (Γ ,,, fix_context mfix0) (Γ' ,,, fix_context mfix1) dtype dbody (fun x => (dname x, rarg x)) P' mfix0 mfix1 ->
+          P Γ Γ' (tCoFix mfix0 idx) (tCoFix mfix1 idx)) ->
+      (forall (Γ Γ' : context) (na : name) (M0 M1 N0 N1 : term),
+          pred1_extra Γ Γ' M0 M1 ->
+          P Γ Γ' M0 M1 -> pred1_extra (Γ,, vass na M0) (Γ' ,, vass na M1) N0 N1 ->
+          P (Γ,, vass na M0) (Γ' ,, vass na M1) N0 N1 -> P Γ Γ' (tProd na M0 N0) (tProd na M1 N1)) ->
+      (forall (Γ Γ' : context) (ev : nat) (l l' : list term),
+          All2_local_env (on_decl pred1_extra) Γ Γ' ->
+          Pctx Γ Γ' ->
+          All2 (P' Γ Γ') l l' -> P Γ Γ' (tEvar ev l) (tEvar ev l')) ->
+      (forall (Γ Γ' : context) (t : term),
+          All2_local_env (on_decl pred1_extra) Γ Γ' ->
+          Pctx Γ Γ' ->
+          pred_atom t -> P Γ Γ' t t) ->
+      forall (Γ Γ' : context) (t t0 : term), pred1_extra Γ Γ' t t0 -> P Γ Γ' t t0.
+  Proof.
+    intros P Pctx P' Hctx.
+    intros X X0 X1 X2 X3 X4 X5 X6 X7 Xrw Xprw Xxrw X8 X9 X10 X11 X12 X13 X14 X15 X16
+      X17 X18 X19 X20 Γ Γ' t t0 X21.
+    revert Γ Γ' t t0 X21.
+    fix aux 5. intros Γ Γ' t t'.
+    move aux at top.
+    destruct 1; match goal with
+                | |- P _ _ (tFix _ _) (tFix _ _) => idtac
+                | |- P _ _ (tCoFix _ _) (tCoFix _ _) => idtac
+                | |- P _ _ (mkApps (tFix _ _) _) _ => idtac
+                | |- P _ _ (tCase _ _ (mkApps (tCoFix _ _) _) _) _ => idtac
+                | |- P _ _ (tProj _ (mkApps (tCoFix _ _) _)) _ => idtac
+                | |- P _ _ (tRel _) _ => idtac
+                | |- P _ _ (tSymb _ _ _) _ => idtac
+                | |- P _ _ (tConst _ _) _ => idtac
+                | lhs := _, rhs := _ |- _ => idtac
+                | H : _ |- _ => eapply H; eauto
+                end.
+    - simpl. apply X1; auto. apply Hctx.
+      + apply (All2_local_env_impl a). intros. eapply X21.
+      + apply (All2_local_env_impl a). intros. eapply (aux _ _ _ _ X21).
+    - simpl. apply X2; auto.
+      apply Hctx, (All2_local_env_impl a).
+      + exact a.
+      + intros. apply (aux _ _ _ _ X21).
+    - apply Hctx, (All2_local_env_impl a). 1: exact a.
+      intros. apply (aux _ _ _ _ X21).
+    - eapply (All2_All2_prop (P:=pred1_extra) (Q:=P') a0 ((extendP aux) Γ Γ')).
+    - eapply (All2_All2_prop_eq (P:=pred1_extra) (Q:=P') (f:=snd) (g:=fst) a1 (extendP aux Γ Γ')).
+    - eapply X4; eauto.
+      + apply Hctx, (All2_local_env_impl a). 1: exact a.
+        intros. apply (aux _ _ _ _ X21).
+      + eapply (All2_local_env_impl a0). intros. red. red in X21.
+        apply (aux _ _ _ _ X21).
+      + eapply (All2_All2_prop2_eq (Q:=P') (f:=dtype) (g:=dbody) a1 (extendP aux)).
+      + eapply (All2_All2_prop (P:=pred1_extra) (Q:=P') a2 (extendP aux Γ Γ')).
+    - eapply X5; eauto.
+      + apply Hctx, (All2_local_env_impl a). 1: exact a.
+        intros. apply (aux _ _ _ _ X22).
+      + eapply (All2_local_env_impl a0). intros. red. red in X22.
+        apply (aux _ _ _ _ X22).
+      + eapply (All2_All2_prop2_eq (Q:=P') (f:=dtype) (g:=dbody) a1 (extendP aux)).
+      + eapply (All2_All2_prop (P:=pred1_extra) (Q:=P') a2 (extendP aux Γ Γ')).
+      + eapply (All2_All2_prop_eq (P:=pred1_extra) (Q:=P') (f:=snd) a3 (extendP aux Γ Γ')).
+    - eapply X6; eauto.
+      + apply Hctx, (All2_local_env_impl a). 1: exact a.
+        intros. apply (aux _ _ _ _ X21).
+      + eapply (All2_local_env_impl a0). intros. red. red in X21. apply (aux _ _ _ _ X21).
+      + eapply (All2_All2_prop2_eq (Q:=P') (f:=dtype) (g:=dbody) a1 (extendP aux)).
+      + eapply (All2_All2_prop (P:=pred1_extra) (Q:=P') a2 (extendP aux Γ Γ')).
+    - eapply X7. 1: assumption.
+      apply Hctx, (All2_local_env_impl a).
+      + intros. exact a.
+      + intros. apply (aux _ _ _ _ X21).
+    - eapply Xrw. all: eauto.
+      + apply Hctx. 1: auto.
+        apply (All2_local_env_impl a). intros. apply (aux _ _ _ _ X21).
+      + eapply (All2_All2_prop (P:=pred1_extra) (Q:=P') a0 ((extendP aux) Γ Γ')).
+    - eapply Xprw. all: eauto.
+      + apply Hctx. 1: auto.
+        apply (All2_local_env_impl a). intros. apply (aux _ _ _ _ X21).
+      + eapply (All2_All2_prop (P:=pred1_extra) (Q:=P') a0 ((extendP aux) Γ Γ')).
+    - eapply Xxrw. all: eauto.
+      + apply Hctx. 1: auto.
+        apply (All2_local_env_impl a). intros. apply (aux _ _ _ _ X21).
+      + eapply (All2_All2_prop (P:=pred1_extra) (Q:=P') a0 ((extendP aux) Γ Γ')).
+    - eapply X8; eauto.
+      apply Hctx, (All2_local_env_impl a).
+      + intros. exact a.
+      + intros. apply (aux _ _ _ _ X21).
+    - eapply X9; eauto.
+      apply Hctx, (All2_local_env_impl a). 1: exact a.
+      intros. apply (aux _ _ _ _ X21).
+    - apply Hctx, (All2_local_env_impl a). 1: exact a.
+      intros. apply (aux _ _ _ _ X21).
+    - eapply (All2_All2_prop (P:=pred1_extra) (Q:=P) a0). intros. apply (aux _ _ _ _ X21).
+    - eapply (All2_All2_prop_eq (P:=pred1_extra) (Q:=P') (f:=snd) a (extendP aux Γ Γ')).
+    - eapply X16.
+      + eapply (All2_local_env_impl a). intros. apply X21.
+      + eapply (Hctx _ _ a), (All2_local_env_impl a). intros. apply (aux _ _ _ _ X21).
+      + eapply (All2_local_env_impl a0). intros. red. exact X21.
+      + eapply (All2_local_env_impl a0). intros. red. apply (aux _ _ _ _ X21).
+      + eapply (All2_All2_prop2_eq (Q:=P') (f:=dtype) (g:=dbody) a1 (extendP aux)).
+    - eapply X17.
+      + eapply (All2_local_env_impl a). intros. apply X21.
+      + eapply (Hctx _ _ a), (All2_local_env_impl a). intros. apply (aux _ _ _ _ X21).
+      + eapply (All2_local_env_impl a0). intros. red. exact X21.
+      + eapply (All2_local_env_impl a0). intros. red. apply (aux _ _ _ _ X21).
+      + eapply (All2_All2_prop2_eq (Q:=P') (f:=dtype) (g:=dbody) a1 (extendP aux)).
+    - eapply (Hctx _ _ a), (All2_local_env_impl a). intros. apply (aux _ _ _ _ X21).
+    - eapply (All2_All2_prop (P:=pred1_extra) (Q:=P') a0 (extendP aux Γ Γ')).
+    - eapply (Hctx _ _ a), (All2_local_env_impl a). intros. apply (aux _ _ _ _ X21).
+  Defined.
+
+End ParallelReductionExtra.
+
+Notation pred1_extra_ctx Σ e Γ Γ' :=
+  (All2_local_env (on_decl (pred1_extra Σ e)) Γ Γ').
+
+Lemma pred1_pred1_extra :
+  ∀ Σ Γ Δ u v e,
+    pred1 Σ Γ Δ u v →
+    pred1_extra Σ e Γ Δ u v.
+Proof.
+  intros Σ Γ Δ u v e h.
+  set (Pctx :=
+    fun Γ Δ =>
+      pred1_extra_ctx Σ e Γ Δ
+  ).
+  revert Γ Δ u v h.
+  refine (pred1_ind_all_ctx Σ _ Pctx _ _ _ _ _ _ _ _ _ _ _ _ _ _ _ _ _ _ _ _ _ _ _ _ _).
+  all: try solve [ auto ].
+  all: try solve [ econstructor ; eauto ].
+  all: try solve [
+    intros ;
+    econstructor ; eauto ;
+    solve [ eapply All2_impl ; intuition eauto ; intuition eauto ]
+  ].
+  (* all: try solve [
+    intros ;
+    econstructor ; eauto ;
+    unfold on_Trel in * ;
+    solve [ eapply All2_impl ; intuition eauto ; intuition eauto ]
+  ]. *)
+  all: intros.
+  - econstructor. all: eauto.
+    + eapply All2_impl. 1: eauto.
+      intros ? ? [? [[? ?] ?]]. intuition eauto.
+      unfold on_Trel in *. intuition eauto.
+    + eapply All2_impl. 1: eauto.
+      intros ? ? [? ?]. auto.
+  - econstructor. all: eauto.
+    + eapply All2_impl. 1: eauto.
+      intros ? ? [[? ?] [[? ?] ?]]. unfold on_Trel.
+      intuition eauto.
+    + eapply All2_impl. 1: eauto.
+      intros ? ? [? ?]. auto.
+    + eapply All2_impl. 1: eauto.
+      intros ? ? [[? ?] ?]. intuition auto.
+  - econstructor. all: eauto.
+    + eapply All2_impl. 1: eauto.
+      intros ? ? [[? ?] [[? ?] ?]]. unfold on_Trel.
+      intuition eauto.
+    + eapply All2_impl. 1: eauto.
+      intros ? ? [? ?]. auto.
+  - econstructor. all: eauto.
+    eapply All2_impl. 1: eauto.
+    intros ? ? [[? ?] [[? ?] ?]]. unfold on_Trel.
+    intuition eauto.
+  - econstructor. all: eauto.
+    eapply All2_impl. 1: eauto.
+    intros ? ? [[? ?] [[? ?] ?]]. unfold on_Trel.
+    intuition eauto.
+Qed.
